examples/sess/examples.v
@@ -1,0 +1,173 @@
+From stdpp Require Import base gmap.
+From mathcomp Require Import ssreflect.
+From stdpp Require Import namespaces.
+From iris.algebra Require Import agree auth csum gset gmap excl frac.
+From iris.algebra Require Import max_prefix_list.
+From iris.heap_lang Require Import notation proofmode.
+From cryptis Require Import lib term gmeta cryptis primitives tactics role.
+From cryptis.examples Require Import iso_dh gen_conn sess.
+(* From crypti *)
+(* From cryptis.examples.sess Require impl. *)
+(* From cryptis.examples.sess.proofs Require Import base. *)
+From actris.channel Require Import proto_model proto.
+From iris.heap_lang Require Import lib.spin_lock.
+From iris.bi Require Import telescopes.
+
+
+Set Implicit Arguments.
+Unset Strict Implicit.
+Unset Printing Implicit Defensive.
+
+Section Send42Example.
+Implicit Types skI skR pkI pkR : sign_key.
+Implicit Types N : namespace.
+
+Context `{!cryptisGS Σ, !heapGS Σ, !iso_dhGS Σ, !GenConn.connGS Σ, !Sess.sessG Σ}.
+Notation iProp := (iProp Σ).
+
+Definition send42_proto : iProto Σ term :=
+  (<!> MSG  (TInt 42); END)%proto.
+
+
+Definition send42_proto_dual : iProto Σ term :=
+  (<?> MSG (TInt 42); END)%proto.
+
+
+Definition initiator_send42 : val :=
+  λ: "c" "skI" "pkR" "tagN",
+    let: "cs" := Sess.connect "c" "skI" "pkR" "tagN" in
+    Sess.send "cs" (TInt 42);;
+    "cs".
+
+Definition responder_recv42 : val :=
+  λ: "c" "skR" "tagN",
+    let: "req" := Sess.listen "c" in
+    let: "cs" := Sess.confirm "c" "skR" "tagN" "req" in
+    let: "msg" := Sess.recv "cs" in
+    ("cs", "msg").
+
+Lemma wp_initiator_send42 c skI skR N :
+  channel c -∗
+  cryptis_ctx -∗
+  Sess.ctx N send42_proto -∗
+  minted skI -∗
+  minted skR -∗
+  {{{ GenConn.failure skI skR ∨ True }}}
+    initiator_send42 c skI (Spec.pkey skR) (Tag N)
+  {{{ cs, RET (repr cs);
+      Sess.connected skI skR Init cs END ∗
+      release_token (si_init_share cs) ∗
+      (public (si_key cs) ∨ True) }}}.
+
+Proof.
+  iIntros "#? #? #? #? #? % !> #P post".
+
+  rewrite /initiator_send42.
+  wp_lam.
+
+  wp_pures.
+  wp_bind (impl.connect _ _ _ _).
+  wp_apply (Sess.wp_connect with "[] [P]"); eauto 10.
+  iIntros " % ( p1 & p2 & p3 )".
+
+
+  wp_pures.
+  wp_apply (Sess.wp_send with "[] [p1]"); eauto 10.
+iIntros.
+wp_seq.
+iModIntro.
+iApply "post".
+by iFrame.
+Qed.
+
+
+Lemma send42_dual_equiv:
+  iProto_dual send42_proto ≡ send42_proto_dual.
+  Proof.
+    unfold send42_proto_dual.
+    Search iProto_dual.
+   Search iMsg_dual.
+    rewrite /send42_proto iProto_dual_message /= iMsg_dual_base  iProto_dual_end.
+    reflexivity.
+    Qed.
+
+(* Lemma connected_send42_proper skI skR rl cs: *)
+
+
+
+Lemma wp_responder_recv42 c skI skR N :
+  channel c -∗
+  cryptis_ctx -∗
+  Sess.ctx N send42_proto -∗
+  minted skI -∗
+  minted skR -∗
+  {{{ True }}}
+    responder_recv42 c skR (Tag N)
+  {{{ cs msg, RET (repr cs, msg);
+      Sess.connected skR skI Resp cs END ∗
+      release_token (si_resp_share cs) ∗
+      (public (si_key cs) ∨ True) ∗
+      ⌜msg = TInt 42⌝ }}}.
+
+Proof.
+  iIntros "#? #? #? #HskI #HskR % !> #P post".
+  rewrite /responder_recv42.
+  wp_lam.
+    wp_pures.
+    wp_bind (impl.listen _).
+    wp_apply (Sess.wp_listen with "[] [P]"); eauto 10.
+    (* iIntros. *)
+    iIntros (ga skI0) "[#Hpub #Hmint]".
+    wp_pures.
+    wp_bind (impl.confirm _ _ _ _).
+    wp_apply (Sess.wp_confirm True with "[] [P]"); eauto 10.
+    (* iFrame " Hmint Hpub HskR". *)
+    (* iRight. *)
+
+    iIntros (cs) "[Hconn H']".
+    wp_pures.
+    wp_bind (impl.recv _).
+    (* rewrite /send42_proto_dual /iProto_dual /=. *)
+
+    Search iProto_dual.
+    wp_apply (@Sess.wp_recv
+            (* (TT := tele_unit) *)
+            (* (skI := skI0) (skR := skR) (rl := Resp) (cs := cs) *)
+            (* (N := N) (p0 := send42_proto) *)
+            (* (t := λ _, TInt 42) *)
+            (* (P := λ _, True%I) *)
+                _ _ _ _ _ _
+                _             (* TT *)
+                skI0 skR Resp cs N send42_proto
+                (fun _ => TInt 42)
+                (fun _ => True%I)
+                (fun _ => END)
+          with "[] [Hconn]"); eauto 10.
+    (* wp_apply (Sess.wp_recv with "[] [Hconn]"); eauto 10. *)
+    (* rewrite send42_proto iProto_dual_message. *)
+    (* unfold send42_proto. *)
+    simpl.
+    Search iProto_dual.
+    Existing Instance Sess.connected_proper.
+    (* iEval (rewrite /base.connected; rewrite [iProto_dual send42_proto]helper) in "Hconn". *)
+    (* rewrite /send42_proto  helper. *)
+    (* rewrite /send42_proto iProto_dual_message . /= iMsg_dual_base  iProto_dual_end. *)
+    (* rewrite helper in "Hconn". *)
+    (* iAssert (base.connected skI0 skR Resp cs send42_proto_dual) with "[Hconn]" as "Hconn". *)
+(* { rewrite -send42_dual_equiv. *)
+
+    (* iEval (rewrite send42_dual_equiv) in "Hconn". *)
+    rewrite send42_dual_equiv .
+    unfold send42_proto_dual.
+    (* iExact "Hconn". *)
+    (* iApply "Hconn". *)
+    iFrame "Hconn".
+
+
+    (* } *)
+
+
+
+
+
+End Send42Example.
